small syntax changes for improved readability

uc-dsl/examples/megan/pke_ind_cpa.ec
@@ -14,27 +14,28 @@ type ciphertext.
 (* randomness *)
 type rand.
 op drand : rand distr.
-axiom dexp_uni : is_uniform drand.
-axiom dexp_fu : is_full drand.
+axiom drand_uni : is_uniform drand.
+axiom drand_fu : is_full drand.
 axiom drand_ll  : is_lossless drand.
-
-op ciph_def : ciphertext.  (* default ciphertext *)
 
 (* Encryption scheme algorithms *)
 op dkeygen : (pkey * skey) distr.
 axiom keygen_ll: is_lossless dkeygen.
 (* what other axioms on dkeygen? *)
+
+pred valid_keys (keys: pkey * skey) = support dkeygen keys.
+
 op enc(pk:pkey, m:plaintext, r:rand) : ciphertext.
 op dec(sk:skey, c:ciphertext) : plaintext.
 
 (* For checking correctness of encryption scheme *)
 axiom correctness (pk: pkey, sk: skey, m: plaintext, r : rand):
-  support dkeygen (pk, sk) =>
+  valid_keys (pk, sk) =>
   dec sk (enc pk m r) = m.
 
 module type ADV_INDCPA = {
   (* choose a pair of plaintexts *)
-  proc choose(pk : pkey): plaintext * plaintext 
+  proc choose(pk : pkey): plaintext * plaintext
 
   (* guess which plaintext was encrypted *)
   proc guess(c : ciphertext): bool
@@ -43,10 +44,10 @@ module type ADV_INDCPA = {
 (* IND-CPA Security Game, parametrized by an encryption scheme Enc and ind-cpa adversary *)
 module INDCPA (Adv : ADV_INDCPA) = {
   proc main() : bool = {
-    var b, b' : bool; 
-    var x1, x2 : plaintext; 
-    var c : ciphertext; 
-    var r : rand; 
+    var b, b' : bool;
+    var x1, x2 : plaintext;
+    var c : ciphertext;
+    var r : rand;
     var pk : pkey; var sk : skey;
 
     (pk, sk) <$ dkeygen;         (* generate keys for PKE *)
